smtlink/z3_interface/RewriteExpt.py
@@ -28,6 +28,8 @@ class to_smt_w_expt(ACL22SMT.to_smt):
         # the translator turns integerp to isReal!  That's because the z3
         # solver (understandably) chokes on mixed integer/real polynomials.
         self.expt = z3.Function('expt', z3.RealSort(), z3.RealSort(), z3.RealSort())
+        self.b_sum = z3.Function('b_sum', z3.RealSort(), z3.RealSort(), z3.RealSort(), z3.RealSort(), z3.RealSort(), z3.RealSort(), z3.RealSort())
+        self.b_expt = z3.Function('b_expt', z3.RealSort(), z3.RealSort(), z3.RealSort())
         self.maxPowExpand = 10
 
     def simplify(self, expr, **kwargs):
