mark-smtlink/config.lisp
@@ -3,13 +3,40 @@
 ;; 2. Z3_files
 ;; 3. name of z3 class
 ;; 4. SMT command
-
 (in-package "ACL2")
-(defconst *dir-interface* "/Users/mrg/src/smtlink/smtlink/z3\_interface")  ;; mrg
-(defconst *dir-files* "z3\_files")
-;; (defconst *z3-module* "ACL2\_translator") ;; mrg changed to use my subclass
-(defconst *z3-module* "RewriteExpt")
+(include-book "std/util/defaggregate" :dir :system)
+
+(std::defaggregate smtlink-config
+  (dir-interface
+   dir-files
+   SMT-module
+   SMT-class
+   smt-cmd
+   dir-expanded)
+  :tag :smtlink-config)
+
+(defconst *default-smtlink-config*
+  (make-smtlink-config :dir-interface "./"
+		       :dir-files "z3\_files" 
+		       :SMT-module "ACL22SMT"
+		       :SMT-class "to_smt"
+		       :smt-cmd "python"
+		       :dir-expanded  "expanded"))
+
+(encapsulate
+  (((smt-cnf) => *))
+  (local (defun smt-cnf ()
+	   *default-smtlink-config*)))
+
+(defun default-smtlink-config ()
+  (declare (xargs :guard t))
+  (change-smtlink-config *default-smtlink-config*))
+
+(defattach smt-cnf default-smtlink-config)
+
+;; (defconst *dir-interface* "/ubc/cs/home/y/yanpeng/project/ACL2/smtlink/z3\_interface")
+;; (defconst *dir-files* "z3\_files")
+;; (defconst *z3-module* "ACL22SMT")
 ;; (defconst *z3-class* "to_smt")
-(defconst *z3-class* "to_smt_w_expt")
-(defconst *smt-cmd* "python")
-(defconst *dir-expanded* "expanded")
+;; (defconst *smt-cmd* "python")
+;; (defconst *dir-expanded* "expanded")
